Working on subtyping PER

theories/PtsSignature.v
@@ -18,13 +18,20 @@ Inductive st_subtyp {P : PtsSig} : P -> P -> Prop :=
 | st_subtyp_trans : forall s1 s2 s3, Ax_sub P s1 s2 -> st_subtyp s2 s3 ->
                                 st_subtyp s1 s3.
 
+#[export]
+Instance st_subtyp_transtive {P} : Transitive (@st_subtyp P).
+Proof.
+  induction 1; intros; eauto.
+  econstructor; eauto.
+Qed.
+
 Record PredicativeSig (P : PtsSig) : Type :=
   mkPredicativeSig {
       pred_rel : relation P;
       ord_rel : StrictOrder pred_rel;
       wf_rel : well_founded pred_rel;
       ord_ax_typ : forall {s1 s2 : P}, Ax_typ P s1 s2 -> pred_rel s1 s2;
-      resp_by_sub : forall {s1 s2 : P}, Ax_sub P s1 s2 -> pred_rel s1 s2;
+      ord_ax_sub : forall {s1 s2 : P}, Ax_sub P s1 s2 -> pred_rel s1 s2;
       ord_ru_pi : forall {s1 s2 s3 : P}, Ru_pi P s1 s2 s3 -> (pred_rel s1 s3 \/ s1 = s3) /\ (pred_rel s2 s3 \/ s2 = s3);
 
     }.
@@ -33,7 +40,47 @@ Arguments ord_rel {_}.
 Arguments wf_rel {_}.
 Arguments ord_ax_typ {_} _ {_ _}.
 Arguments ord_ru_pi {_} _ {_ _ _}.
-Arguments resp_by_sub {_} _ {_ _}.
+Arguments ord_ax_sub {_} _ {_ _}.
+
+Lemma ord_st_subtyp {P} (pred_P : PredicativeSig P) : forall {s1 s2 : P}, st_subtyp s1 s2 -> (pred_rel pred_P s1 s2 \/ s1 = s2).
+Proof.
+  induction 1.
+  - right; reflexivity.
+  - assert (pred_rel pred_P s1 s2) by (eapply ord_ax_sub; eauto).
+    assert (Transitive (pred_rel pred_P)) by (eapply (ord_rel pred_P)).
+    left.
+    destruct IHst_subtyp; [transitivity s2 | subst]; eauto.
+Qed.
+
+Lemma ord_ax_typ_sub {P} (pred_P : PredicativeSig P) : forall {s1 s2 s3 : P}, Ax_typ P s1 s2 -> st_subtyp s2 s3 -> pred_rel pred_P s1 s3.
+Proof.
+  intros.
+  assert (Transitive (pred_rel pred_P)) by (eapply (ord_rel pred_P)).
+  assert (pred_rel pred_P s1 s2) by (eapply ord_ax_typ; eauto).
+  assert (pred_rel pred_P s2 s3 \/ s2 = s3) by (eapply ord_st_subtyp; eauto).
+  destruct H3.
+  - transitivity s2; eauto.
+  - subst; eauto.
+Qed.
+
+Lemma ord_ru_pi_sub {P} (pred_P : PredicativeSig P) : forall {s1 s2 s3 s3'}, Ru_pi P s1 s2 s3 -> st_subtyp s3 s3' -> (pred_rel pred_P s1 s3' \/ s1 = s3') /\ (pred_rel pred_P s2 s3' \/ s2 = s3').
+Proof.
+  intros.
+  assert (Transitive (pred_rel pred_P)) by (eapply (ord_rel pred_P)).
+  eapply (ord_ru_pi pred_P) in H as [].
+  eapply (ord_st_subtyp pred_P) in H0.
+  split.
+  - destruct H; destruct H0.
+    + left; transitivity s3; eauto.
+    + left; subst; eauto.
+    + left; subst; eauto.
+    + right; subst; eauto.
+  - destruct H2; destruct H0.
+    + left; transitivity s3; eauto.
+    + left; subst; eauto.
+    + left; subst; eauto.
+    + right; subst; eauto.
+Qed.
 
 Section OrderProperties.
   Context {P : PtsSig} (pred_P : PredicativeSig P).
